

$$\partial_x A^2 = -P' \underbrace{\frac{2x x_R^2}{(x^2 + x_R^2)^2}}_{f(x)} \underbrace{\left[1 - \frac{2r^2 x_R^2}{\omega_0^2 (x^2 + x_R^2)} \right]}_{g(x)} \underbrace{\exp\left(-\frac{2r^2 x_R^2}{\omega_0^2 (x^2 + x_R^2)}\right)}_{h(x)}$$

$$f(x) = f(a) + f'(a)(x-a) + \frac{1}{2!} f''(a)(x-a)^2 + \dots$$

$$f'(x) = \frac{(x^2 + x_R^2) 2x_R^2 - 2x^2 x_R^2}{(x^2 + x_R^2)^3}$$

$$g'(x) = \frac{8r^2 x_R^2 x}{\omega_0^2 (x^2 + x_R^2)^2}$$

$$h'(x) = g'(x) h(x)$$

sattelpunkt

↓

$$f''(x) = -\frac{8x_R^2 x}{(x^2 + x_R^2)^3} - \frac{76x x_R^2 (x^2 + x_R^2) - 48x^3 x_R^2}{(x^2 + x_R^2)^3}$$

$$g''(x) = \frac{8r^2 x_R^2 (x^2 + x_R^2) - 32r^2 x_R^2 x^2}{\omega_0^2 (x^2 + x_R^2)^3}$$

$$h''(x) = g''(x) h(x) + g'(x)^2 h(x)$$

$$\partial_x A^2 = \partial_x A(a) + (x-a) [f'(a)g(a)h(a) + g'(a)f(a)h(a) + g'(a)h(a)g(a)f(a)]$$

$$+ \frac{1}{2!} \underbrace{(x-a)^2}_{\tilde{x}^2} \left[f''(a)g(a)h(a) + f'(a)g'(a)h(a) + f'(a)g(a)h'(a) \right. \quad \wedge$$

$$+ g''(a)f(a)h(a) + g'(a)f'(a)h(a) + g'(a)^2 f(a)h(a) \quad \text{minimi poig}$$

korrektur
minuten →

$x \rightarrow x - x_0$

$$+ g''(a)h(a)f(a)g(a) + g'(a)^2 h(a)f(a)g(a) + g'(a)h(a)g(a)f(a) \left. \right] + \dots$$



Saa lauan $p \approx -m\Omega^2 x + \dots$

$$V = \frac{1}{2} \hat{\Omega}^2 m \tilde{x}^2 \quad \hat{\Omega}^2 = \frac{1}{m} \left. \frac{\partial^2 V}{\partial x^2} \right|_{x=x_0}$$

Tarkista p-luotessa $V = \frac{1}{2} \hat{\Omega}^2 m \tilde{x}^2$

että saa oikean muodon

